hol: state machines, before I remove carrier

HOL/testItreeScript.sml
@@ -33,13 +33,13 @@
 open stringLib; (* parsing, text examples etc. *)
 open itreeTauTheory;
 
+open relationTheory bisimulationTheory;
+open pathTheory;
+
 Overload emit[local] = “itree_trigger”;
 val _ = temp_set_fixity ">>=" (Infixl 500);
 Overload ">>="[local] = “itree_bind”;
 Overload iter[local] = “itree_iter”;
-
-val _ = temp_set_fixity "≈" (Infixl 500);
-Overload "≈" = “itree_wbisim”;
 
 (* open monadsyntax; *)
 (* val _ = *)
@@ -50,10 +50,283 @@ Overload "≈" = “itree_wbisim”;
 (*     ) *)
 (* val _ = monadsyntax.temp_enable_monad "itree_monad"; *)
 
+val _ = temp_set_fixity "≈" (Infixl 500);
+Overload "≈" = “itree_wbisim”;
+
+(*
+ * state predicate, transition relation, initial state, success predicate
+ *)
+Type lts[pp] = “:((α -> bool) # (α # β option # α -> bool) # α)”;
+
+Definition lts_states[simp]:
+  lts_states ((c,r,i) : ('s,'a) lts) = c
+End
+Definition lts_rel[simp]:
+  lts_rel ((c,r,i) : ('s,'a) lts) = r
+End
+Definition lts_init[simp]:
+  lts_init ((c,r,i) : ('s,'a) lts) = i
+End
+
+Definition curry3[simp]:
+  curry3 P = λa b c. P (a,b,c)
+End
+Definition uncurry3[simp]:
+  uncurry3 Q = λ(a,b,c). Q a b c
+End
+
+(* CSP || operator
+ *
+ * note: the LTS event type is more general than (e,a)
+ * note: competing processes should not communicate directly
+ *
+ * TODO shallow-embedded channel syntax
+ *)
+
+Definition comm_rel_l:
+  comm_rel_l com r = { ((s,t), a, (s',t')) | a ∉ com ∧ (s,a,s') ∈ r ∧ t = t' }
+End
+
+Definition comm_rel_r:
+  comm_rel_r com r' = { ((s,t), a, (s',t')) | a ∉ com ∧ (t,a,t') ∈ r'∧ s = s' }
+End
+
+Definition comm_rel_com:
+  comm_rel_com com r r' = { ((s,t), a, (s',t')) | a ∉ com ∧ (t,a,t') ∈ r'∧ s = s' }
+End
+
+Definition comm_rel:
+  comm_rel com r r' = comm_rel_l com r ∪ comm_rel_r com r' ∪ comm_rel_com com r r'
+End
+
+Definition comm:
+  comm com ((c,r,i) : ('s,'a) lts) ((c',r',i') : ('t,'a) lts) =
+  ({ (s,s') | c s ∧ c' s'}, comm_rel com r r', (i,i'))
+End
+
+Definition par:
+  par l1 l2 = comm ∅ l1 l2
+End
+
+Definition prefix:
+  prefix i' a ((c,r,i) : ('s,'a) lts) = (c ∪ {i'}, r ∪ {(i',a,i)},i')
+End
+
+(* this is more natural than restriction *)
+Definition hide:
+  hide ((c,r,i) : ('s,'a) lts) a =
+  (c,{ (s,NONE,s') | (s,a,s') ∈ r } ∪ { (s,a',s') | a' ≠ a ∧ (s,a',s') ∈ r }, i)
+End
+
+Definition choice_ext:
+  choice_ext s a ((c,r,i) : ('s,'a) lts) a' ((c',r',i') : ('s,'a) lts) =
+  ({s} ∪ c ∪ c', r ∪ { (s,a,i); (s,a',i') }, s)
+End
+
+Definition choice_int:
+  choice_int s l1 l2 = choice_ext s NONE l1 NONE l2
+End
+
+(* monad *)
+Definition seq:
+  seq ((c,r,i) : ('s,'a) lts) (final : 's -> bool) (next : 's -> ('s,'a) lts) =
+  (c ∪ BIGUNION { lts_states (next s) | final s },
+   r ∪ { (fs,NONE,lts_init (next fs)) | final fs }
+     ∪ BIGUNION { lts_rel (next s) | final s },
+   i)
+End
+
+Definition fix:
+  fix ((c,r,i) : ('s,'a) lts) (final : 's -> bool)
+  = seq (c,r,i) final (K (c,r,i))
+End
+
+(* the equivalence of choice: weak bisimulation, a congruence for csp
+ * more fine than trace equivalence for dealing with liveness
+ *)
+
+Definition curry3[simp]:
+  curry3 r = (λs a s'. (s,a,s') ∈ r)
+End
+
+Definition lts_wbisim:
+  lts_wbisim r s t = WBISIM_REL (curry3 r) NONE s t
+End
+
+(* XXX can't enable types *)
+Theorem lts_wbisim_refl[simp]:
+  lts_wbisim r s s
+Proof
+  rw[lts_wbisim] >>
+  metis_tac[WBISIM_REL_IS_EQUIV_REL, equivalence_def, reflexive_def]
+QED
+
+Theorem lts_wbisim_sym:
+  lts_wbisim r s t ⇒ lts_wbisim r t s
+Proof
+  rw[lts_wbisim] >>
+  metis_tac[WBISIM_REL_IS_EQUIV_REL, equivalence_def, symmetric_def]
+QED
+
+Theorem lts_wbisim_trans:
+  lts_wbisim r s t ∧ lts_wbisim r t u ⇒ lts_wbisim r s u
+Proof
+  rw[lts_wbisim] >>
+  metis_tac[WBISIM_REL_IS_EQUIV_REL, equivalence_def, transitive_def]
+QED
+
+(*
+ * example interpreting itrees into labelled transition systems
+ *)
+CoInductive subtree:
+[~tau:]
+  (subtree t s ⇒ subtree (Tau t) s)
+[~vis:]
+  (subtree (k a) s ⇒ subtree (Vis e k) s)
+[~id:]
+  (subtree t t)
+End
+
+Theorem subtree_trans:
+  subtree s r ∧ subtree t s ⇒ subtree t r
+Proof
+  strip_tac >>
+  irule subtree_coind >>
+  qexists_tac ‘λt' r'. ∃s'. subtree t' s' ∧ subtree s' r'’ >>
+  reverse (rw[]) >- (metis_tac[]) >>
+  ntac 2 (last_x_assum kall_tac) >>
+  Cases_on ‘a0’ >> metis_tac[subtree_cases]
+QED
+
+Inductive itree_rel:
+  itree_rel (Tau t, NONE, t) ∧
+  itree_rel (Vis e k, SOME (e,a), (k a))
+End
+
+Definition itree_sm_def:
+  itree_sm (t : ('a,'e,'r) itree)
+  = (subtree t,
+     itree_rel : ('a,'e,'r) itree # ('e # 'a) option # ('a,'e,'r) itree -> bool,
+     t)
+End
+
+(* lts predicates *)
+
+CoInductive lts_globally:
+  (∀s' a. (s,a,s') ∈ r ⇒ P (s,a,s') ∧ lts_globally r P s')
+  ⇒ lts_globally r P s
+End
+
+Inductive lts_future:
+  (∀s a. (s,a,s') ∈ r ⇒ P (s,a,s') ∨ lts_future r P s')
+  ⇒ lts_future r P s
+End
+
+(* TODO preservation under weak bisimulation
+ * TODO syntax for transitions s -r-> s' and weak bisimilarity s ≈r≈ s
+ * P must respect weakly bisimilar states
+ *)
+
+Theorem globally_resp_wbisim:
+  lts_wbisim (r ∪ r') s s' ∧ (∀s s'. P (s,NONE,s'))
+  ⇒ lts_globally r P s ⇒ lts_globally r' P s'
+Proof
+  cheat
+QED
+
+(* the producer produces buffers (represented as numbers / pointers)
+ * and can sometimes stop in the false state.
+ * Meanwhile the consumer receives and sends them
+ *)
+
+Datatype:
+  testev = Produce num | Recv | Send num
+End
+
+Definition prod_def:
+  prod = (K T, { (T,SOME(Recv,Produce n),T) | n < 256 } ∪ {(T,NONE,F)}, T)
+         : (bool, testev # testev) lts
+End
+
+(* sanity check: we can continuously produce the 0 pointer *)
+Theorem test_okpath:
+  okpath (curry3 (lts_rel prod))
+         (unfold (λ_. T) (λ_. SOME ((),SOME (Recv,Produce 0))) ())
+Proof
+  irule okpath_unfold >>
+  qexists_tac ‘K T’ >>
+  rw[prod_def]
+QED
+
+Definition prod_extract[simp]:
+  prod_extract (Produce n) = n
+End
+
+Definition csm_tree_def:
+  csm_tree = itree_iter (λ_. Vis Recv
+                                 (λa. Vis (Send (prod_extract a))
+                                          (λ_. Ret (INL ()))))
+                        ()
+End
+
+(* FINAL linear correctness statement *)
+Definition prod_csm_com:
+  prod_csm_com = { SOME (Recv,Produce n) | n < 256 }
+End
+
+Definition sys_def[simp]:
+  sys = comm prod_csm_com prod (itree_sm csm_tree)
+End
+
+Theorem comm_rel_r_lift:
+  ((s,t),a,(s',t')) ∈ comm_rel_r com r' ⇔ a ∉ com ∧ (t,a,t') ∈ r' ∧ s = s'
+Proof
+  rw[comm_rel_r] >> metis_tac[]
+QED
+
+Theorem correspondence:
+  lts_wbisim (comm_rel com r r')
+Proof
+QED
+
+(* XXX types are wrong *)
+Theorem correctness:
+  lts_globally sys
+  (λ(s,a,s'). prod_csm_com a
+              ⇒ (lts_future sys (λ(s,a,s'). ∃x. a = SOME (Send n,x)) s'))
+  (lts_init sys)
+Proof
+QED
+
+(* TODO can extend to statement about traces *)
+
+Definition allpaths:
+  allpaths lts P = (∀path. okpath (curry3 (lts_rel lts)) path ⇒ P path)
+End
+
+Definition nowlike:
+  nowlike f p = ∃x. first_label p = f x
+End
+
+CoInductive globally:
+  (P (pcons s a p) ∧ globally P p) ⇒ globally P (pcons s a p)
+End
+
+Inductive future:
+  (∀P p. P p ⇒ future P p) ∧
+  (∀s a P p. future P p ⇒ future P (pcons s a p))
+End
+
+
+
+
+
+
+
 (* Theorem test: *)
 (*   (∀x y. V(i(x,i(y,x)))) ∧ *)
 (*   (∀x y z. V(i(i(x,i(y,z)), i(i(x,y),i(x,z))))) ∧ *)
-(*   (∀x y. V(i(i(y,x),i(n(x),n(y))))) ∧ *)
+(*   (* (∀x y. V(i(i(y,x),i(n(x),n(y))))) ∧ *) *)
 (*   (∀x y. V(i(x,y)) ∧ V(x) ⇒ V(y)) *)
 (*   ⇒ *)
 (*   V(i(a,i(i(a,b),b))) *)
@@ -61,75 +334,71 @@ Overload "≈" = “itree_wbisim”;
 (*   metis_tac[] *)
 (* QED *)
 
+(* (* parallel compose itrees *)
+(*  * separate type of completed communications *)
+(*  * the presence of true nondet is messy *)
+(*  *) *)
 
+(* Datatype: *)
+(*   message = Comm 'a 'a | Call 'a | Select | Choice num *)
+(* End *)
 
+(* Definition call_def: *)
+(*   call (Call a) = a *)
+(* End *)
 
+(* Definition is_com_def: *)
+(*   is_com com (Call e) (Call e') = com e e' ∧ *)
+(*   is_com _ _ _ = F *)
+(* End *)
 
-(* state machine:
- * states: S, S × S transition relation
- *)
+(* Type comtree[pp] = “:(α message, α message, β option) itree”; *)
 
-Inductive future_def:
-  (P e ⇒ future P (Vis e k)) ∧
-  (future P t ⇒ future P (Tau t))
-End
+(* Definition select3_def: *)
+(*   select3 t t' t'' = Vis Select *)
+(*                          (λcb. case cb of *)
+(*                                  Choice n => if n = 0 then t *)
+(*                                              else if n = 1 then t' *)
+(*                                              else if n = 2 then t'' *)
+(*                                              else Ret (INR NONE) *)
+(*                                | _ => ARB) *)
+(* End *)
 
-Definition select2_def:
-  select2 t t' = (Vis NONE (λb. if b then t else t'))
-End
-
-Definition par:
-  par com (Vis e k) (Vis e' k')
-  = (if com e e'
-     then par com (k NONE) (k' (THE e))
-     else select2 (Vis e (λa. par com (k a) (Vis e' k')))
-                  (Vis e' (λa. par com (Vis e k) (k' a))))
-  ∧
-  par com (Tau t) (Vis e k) =
-End
-
-Datatype:
-  message = Quit | Data
-End
-
-Definition dev:
-  dev = itree_unfold (λseed.
-                        if seed = NONE
-                        then Vis' NONE (λb. if b then (SOME Data) else (SOME Quit))
-                        else Vis' seed (λ_. NONE))
-                     NONE
-End
-
-Datatype:
-  status = Exited | Emit message | Read
-End
-
-Definition drv:
-  drv = itree_unfold (λstatus.
-                        case status of
-                          Read => Vis' (SOME Read) (λinput.
-                                                      if input = Quit
-                                                      then Exited
-                                                      else Emit input)
-                        | Emit input => Tau' Read
-                        | Exited => Ret' ())
-                     Read
-End
-
-
-
-
-
-
-
-
-
-
-
-
-
-
-
+(* Definition par: *)
+(*   par com (t : ('x,'y) comtree) (t' : ('x,'y) comtree) = *)
+(*   iter *)
+(*   (λseed. *)
+(*      case seed of *)
+(*        (Ret NONE, t) => Ret (INR NONE) *)
+(*      | (t, Ret NONE) => Ret (INR NONE) *)
+(*      | (Ret (SOME r), Ret (SOME r')) => Ret (INR (SOME (r, r'))) *)
+(*      | (Tau t, Tau t') => Ret (INL (t, t')) *)
+(*      | (Ret r, Tau t) => Ret (INL (Ret r, t)) *)
+(*      | (Tau t, Ret r) => Ret (INL (t, Ret r)) *)
+(*      | (Vis e k, Ret r) => Vis (Call (call e)) (λa. Ret (INL (k a, Ret r))) *)
+(*      | (Ret r, Vis e k) => Vis (Call (call e)) (λa. Ret (INL (Ret r, k a))) *)
+(*      | (Vis e k, Tau t) => (select3 *)
+(*                             (Vis (Call (call e)) (λa. Ret (INL (k a, t)))) *)
+(*                             (Ret (INL (Vis e k, t))) *)
+(*                             (Ret (INR NONE))) *)
+(*      | (Tau t, Vis e k) => (select3 *)
+(*                             (Ret (INL (t, Vis e k))) *)
+(*                             (Vis (Call (call e)) (λa. Ret (INL (t, k a)))) *)
+(*                             (Ret (INR NONE))) *)
+(*      (* maybe synchronize, while remaining open to other processes (can restrict) *) *)
+(*      (* natmaps - quotient by branching *) *)
+(*      | (Vis e k, Vis e' k') *)
+(*        => if is_com com e e' *)
+(*           then (select3 *)
+(*                 (Vis (Comm (call e) (call e')) (λ_. Ret (INL (k e', k' e)))) *)
+(*                 (Vis (Call (call e)) (λa. Ret (INL (k a, Vis e' k')))) *)
+(*                 (Vis (Call (call e')) (λa. Ret (INL (Vis e k, k' a))))) *)
+(*           else (select3 *)
+(*                 (Vis (Call (call e)) (λa. Ret (INL (k a, Vis e' k')))) *)
+(*                 (Vis (Call (call e')) (λa. Ret (INL (Vis e k, k' a)))) *)
+(*                 (Ret (INR NONE))) *)
+(*   ) (t,t') *)
+(* End *)
 
 Definition itree_trigger_def:
   itree_trigger event = Vis event Ret
